java

src/MutableMap/MutableMap.java
@@ -2,3 +2,38 @@
 *  Copyright by the contributors to the Dafny Project
 *  SPDX-License-Identifier: MIT
 *******************************************************************************/
+
+import dafny.DafnySet;
+import dafny.TypeDescriptor
+
+package MutableMap;
+
+public class MutableMap {
+  private m;
+
+  public MutableMap() {
+    m = new ;
+  }
+
+  public static void Put(K k, V v) {
+  }
+
+  public static DafnySet<K> Keys() {
+  }
+
+  public static DafnySet<V> Values() {
+  }
+
+  public static DafnySet<(K,V)> Items() {
+  }
+
+  public static V Find(K k) {
+  }
+
+  public static void Remove(K k) {
+
+  }
+
+  public static int Size() {
+  }
+}
