examples/MutableMap/MutableMapExamples.dfy
@@ -12,17 +12,30 @@ module MutableMapExamples {
 
   method Main() {
     var m := new MutableMap<string,string>();
+    assert m.Keys() == {};
+    assert m.Values() == {};
+    assert m.Items() == {};
     assert m.Size() == 0;
-    assert "testkey" !in m.Keys();
     m.Put("testkey", "testvalue");
-    //assert m.Size() == 1;
-    assert "testkey" in m.Keys();
-    assert "testvalue" in m.Values();
     assert m.Find("testkey") == "testvalue";
-    m.Remove("testkey");
-    assert "testkey" !in m.Keys();
-    m.Put("testkey", "testvalue");
+    assert m.Keys() == {"testkey"};
+    assert m.Values() == {"testvalue"};
+    assert m.Items() == {("testkey", "testvalue")};
+    assert m.Size() == 1;
+    m.Put("testkey", "testvalue2");
+    assert m.Keys() == {"testkey"};
+    assert m.Values() == {"testvalue2"};
+    assert m.Items() == {("testkey", "testvalue2")};
+    m.Put("testkey2", "testvalue2");
+    assert m.Keys() == {"testkey", "testkey2"};
+    assert m.Values() == {"testvalue2"};
+    assert m.Items() == {("testkey", "testvalue2"), ("testkey2", "testvalue2")};
+    assert m.Size() == 2;
     assert "testkey" in m.Keys();
-    //assert m.Size() == 1;
+    assert "testkey2" in m.Keys();
+    m.Remove("testkey");
+    /* assert m.Keys() == {"testkey2"};
+    assert m.Values() == {"testvalue2"};
+    assert m.Items() == {("testkey2", "testvalue2")}; */
   }
 }
